\documentclass[a4paper]{article} 
\usepackage[inline]{enumitem}
\usepackage{tasks}
\settasks{label =â€¢}
\usepackage{enumitem}
\setenumerate{label = \alph*)}
\input{head}
\newcolumntype{Y}[1]{>{\centering\arraybackslash} X{#1}}
\begin{document}

%-------------------------------
%	TITLE SECTION
%-------------------------------

\fancyhead[C]{}
\hrule \medskip % Upper rule
\begin{minipage}{0.295\textwidth} 
\raggedright
\footnotesize
Winston Peng \hfill\\   
50364686 \hfill\\
wpeng2@buffalo.edu
\end{minipage}
\begin{minipage}{0.4\textwidth} 
\centering 
\large 
Homework 2 - Predicates \& Logical Proofs\\ 
\normalsize 
Intro To Discrete Structures, 2021\\ 
\end{minipage}
\begin{minipage}{0.295\textwidth} 
\raggedleft
\today\hfill\\
\end{minipage}
\medskip\hrule 
\bigskip

\section{Translate English To Math - Predicates}
\large Predicates:
\normalsize
\begin{itemize}
    \item \textbf{Sitting(x, y):} x is sitting on y
    \item \textbf{Free(y):} y is free
    \item \textbf{Top(y, z):} y is on top of z
    \item \textbf{Brown(y):} y is brown
    \item \textbf{Black(y):} y is black
\end{itemize}
\large Domains:
\normalsize
\begin{itemize}
    \item domain of x: {a group of people}
    \item domain of y and z: {a set of deck boxes}
\end{itemize}
\large Problems: \\
\smallskip
\normalsize
\underline{Note}: B is a constant. Top(y, B): y is on top of B.
\begin{enumerate}
    \item \textbf{Everyone is sitting on some box.} $\forall x \:\exists y, \: Sitting(x, y)$
    \item \textbf{Every box that is free has nobody sitting on it.} $\forall y \; \neg \exists x, \: Sitting(x, Free(y))$
    \item \textbf{Every box that is brown is free.} $\forall y, \: Brown(y)) \implies Free(y)$
    \item \textbf{Every box that is not black and on top of box B is brown.} $\forall y, \: \neg(Black(y) \land Top(y, B)) \implies Brown(y)$
    \item \textbf{There is a box that is black and not free.} $\exists y, \: Black(y) \land \neg Free(y) $
\end{enumerate}

\bigskip %----------------------------------------

\section{Translate Math To English - Predicates}
\large Predicates:
\normalsize
\begin{itemize}
    \item \textbf{Edge(x, y):} x is connected to y
    \item \textbf{Color(x, z):} x has color z
\end{itemize}
\large Domains:
\normalsize
\begin{itemize}
    \item domain of x and y: {all nodes in a graph},
    \item domain of z: {RED, GREEN, BLUE, YELLOW},
\end{itemize}
\large Problems:
\normalsize
\boldmath
\begin{enumerate}
    \item $\forall x \, \exists y \; Edge(x, y)$ \\
    All nodes in the graph are connected to at least one node in the graph.
    \item $\forall z \, \exists x \; Color(x, z)$ \\
    A node in the graph is RED, GREEN, BLUE, and YELLOW.
    \item $\forall x \forall y \forall z \: (Edge(x, y) \land Color(x, z) \implies \neg Color(y, z))$ \\
    Every box that is RED, GREEN, BLUE, and YELLOW is connected to another box. It is not connected to a box that is RED, GREEN, BLUE, and, YELLOW
    \item $\neg \forall x \; Color(x, YELLOW)$ \\
    Not every node is yellow.
    \item $\forall x \, \exists y \; (Edge(x, y) \land Color(x, BLUE) \implies Color(y, RED) \lor Color(y, GREEN))$ \\
    Every blue node in the graph is connected to a node that is either red or green.
\end{enumerate}
\unboldmath

\bigskip %------------------------------------

\section{Negate Given Statements (Quantifier Negation)}
\begin{enumerate}
    \item \boldmath $\exists x \; (P(x) \lor Q(x))$ \unboldmath
    
    $\neg(\exists x \; (P(x) \lor Q(x)))$ \\
    $\forall x \; \neg (P(x) \lor Q(x))$ \\
    $\forall x \; \neg P(x) \land \neg Q(x)$
    
    \item \boldmath $\forall x \, \exists y \; (P(x) \lor Q(y))$ \unboldmath
    
    $\neg(\forall x \, \exists y \; (P(x) \lor Q(y)))$ \\
    $\exists x \, \forall y \; \neg (P(x) \lor Q(y))$ \\
    $\exists x \, \forall y \; \neg P(x) \land \neg Q(y)$ 
    
    \item \boldmath $\exists x \; (P(x) \land \forall y (P(y) \implies Q(y)))$ \unboldmath 
    
    $\neg (\exists x \; (P(x) \land \forall y (P(y) \implies Q(y))))$ \\
    $\forall x \; \neg (P(x) \land \forall y (P(y) \implies Q(y)))$ \\
    $\forall x \; \neg P(x) \lor \neg(\forall y) \neg (P(y) \implies Q(y))$ \\
    $\forall x \; \neg P(x) \lor \exists y \, P(y) \land \neg Q(y)$
\end{enumerate}

\bigskip %------------------------------------------

\section{Prove With Logical Equivalence Laws (Math)}
% \begin{center}
% \begin{tabularx}{0.8\textwidth}{X X X X}
% % \begin{enumerate}
%     \mutlicolumn{2}{c}{$p \implies q$} & \mutlicolumn{2}{X}{$\neg p \land q$} \\
%     \multicolumn{2}{X}{$q \implies r$} & $\neg(p \land r) \implies s$\\
%     $\neg r$ & $r \implies p$ \\
%     % \hline & \hline \\
%     $\therefore \neg p$ & $\therefore s$
% % \end{enumerate}
% \end{tabularx}
% \end{center}
\begin{enumerate}
\boldmath
    \item  $p \implies q$ \\
    $q \implies r$ \\
    $\neg r$ \\
    \begin{tabularx}{0.1\textwidth}{X}
        \hline
    \end{tabularx}\\
    $\therefore \neg p$
\unboldmath
\smallskip

\begin{tabularx}{0.6\textwidth}{X X}
\toprule
1) $p \implies q$ & Hypothesis\\
2) $q \implies r$ & Hypothesis\\
3) $\neg r$ & Hypothesis\\
4) $p \implies r$ & Hypothetical syllogism (1, 2)\\
5) $\neg p$ & Modus tollens (3, 4)\\
\end{tabularx}

\boldmath
    \item $\neg p \land q$ \\
    $\neg(p \land r) \implies s$ \\
    $r \implies p$ \\
    \begin{tabularx}{0.1\textwidth}{X}
        \hline
    \end{tabularx}\\
    $\therefore s$
\unboldmath

\smallskip

\begin{tabularx}{0.6\textwidth}{X X}
\toprule
1) $\neg p \land q$ & Hypothesis\\
2) $\neg(p \land r) \implies s$ & Hypothesis\\
3) $r \implies p$ & Hypothesis\\
% 4) $p \implies q$ & Conditional\\
% 5) $q$ & Modus ponens (4) \\
4) $\neg p$ & Simplification (1) \\
5) $\neg r$ & Modus tollens (4, 3) \\
6) $\neg \neg(p \lor r) \lor s$ & Conditional \\
7) $(p \lor r) \lor s$ & Double Negation Law \\
8) $s$ & Disjunctive Syllogism (7, 4, 5)
\end{tabularx}
\end{enumerate}

\bigskip %-------------------------------------------------------

\section{Prove Or Disprove With Logical Equivalence Laws (English)}
\begin{center}
\begin{tabularx}{0.8\textwidth}{|X|}
\hline
If it is not windy or not cloudy, then we will visit the nearby town and do shopping \\
If we visit the nearby town, then we'll dine at the restaurant \\
we did not dine at the restaurant. \\ [1ex]

\toprule \\

$\therefore$ It was cloudy \\
\hline
\end{tabularx}
\end{center}

\begin{itemize}
    \item p: It is windy 
    \item q: It is cloudy 
    \item r: Visit the nearby town 
    \item s: Do shopping 
    \item t: Dine at restaurant 
\end{itemize}

\begin{tabularx}{0.6\textwidth}{X X}
\toprule \\
1) $(\neg p \lor \neg q) \implies (r \land s)$ & Hypothesis \\
2) $r \implies t$ & Hypothesis \\
3) $\neg t$ & Hypothesis \\
4) $\neg r$ & Moudus tollens (3, 2) \\
5) $(\neg p \lor \neg q) \implies F$ & Simplification (1) \\
6) $\neg (\neg p \lor \neg q)$ & Modus tollens (5) \\
7) $p \land q$ & DeMorgan's Law \\
8) $p$ & Simplification 
\end{tabularx}

\bigskip %----------------------------

\section{Direct Proof}
\boldmath
\begin{tabularx}{1.0\textwidth}{|X|}
\hline
Prove that \textbf{If x is an even integer, then $x^2 - 6x + 5$ is odd} \\
\hline
\end{tabularx}
\unboldmath
\begin{itemize}
    \item Decomposition of statement to $P(x) \implies Q(x)$
    \begin{itemize}
        \item The domain of $x$ is all integers.
        \item $P(x)$: $x$ is an even integer
        \item $Q(x)$: $x^2 - 6x + 5$ is odd.
    \end{itemize}
\end{itemize}
\smallskip

\textbf{\underline{Proof}:} Assume $x$ is an even integer. \\
Then exists an integer $k$ such that $x = 2k$.  \\
Hence: $(2k)^2 - 6x + 5$ + $4k^2 - 6(2k) + 5$ $2(2)k^2 - 6 * 2k + 5$. \\
Since $k$ is an integer, $4k^2 - 6(2k) + 5$ $2(2)k^2 - 6 * 2k + 5$ is also an integer (call it $j$). \\
So $n^2 - 6x + 5$ has the form $2j + 5$.
Therefore, $n^2 -6x + 5$ is an odd integer. 
% As multiplying anything by $2$ results in 2, everything is even, until you add $5$, as $even + odd = odd$, $x^2 - 6x + 5$ is odd.

\bigskip %--------------------------------------

\section{Prove By Contraposition}
\boldmath
\begin{tabularx}{1.0\textwidth}{|X|}
\hline
Prove that \textbf{If $x$ is an integer and $x^2$ is even, then $x$ is even} \\
\hline
\end{tabularx}
\unboldmath
\begin{itemize}
    \item Decomposition of statement to $P(x) \implies Q(x)$
    \begin{itemize}
        \item The domain of $x$ is all integers.
        \item $P(x)$: $x^2$ is an even integer
        \item $Q(x)$: $x$ is even.
    \end{itemize}
\end{itemize}

\textbf{\underline{Proof}:} Assume $x$ is not an even integer. So $x$ is odd. \\
Then exists an integer $k$ such that $x = 2k + 1$. \\
Hence: $(2k + 1)^{2} = 4k^2 + 4k + 1 = 2(2k^2 + 2k) + 1$ \\
Since $k$ is an integer, $2(2k^2 + 2k) + 1$ is also an integer (call it $j$) \\
So, $n^2$ has the form $2j + 1$ \\
Therefore, $x^2$ is an odd integer, so $x^2$ is not an odd integer. \\
Thus, $\neg Q(n) \implies \neg P(n)$. \\
Then, $P(n) \implies Q(n)$ is also true. \\
\end{document}
